core/Coqlib.v
@@ -3,6 +3,7 @@ Require Export Coq.ssr.ssrbool.
 Require Export Coq.micromega.Lia.
 Require Export Coq.Logic.FunctionalExtensionality.
 Require Export Poulet4.Utils.Utils.
+Require Export Coq.ZArith.BinInt.
 Require Export Coq.ZArith.Zcomplements.
 Require Export VST.zlist.Zlist.
 Export ListNotations.
@@ -45,3 +46,63 @@ Inductive Forall2_fold {A B C} (P : A -> B -> C -> A -> Prop) : A -> list B -> l
 
 (* We accept this axiom. Maybe it's avoidable but it makes things simpler by accepting it. *)
 Axiom prop_ext : ClassicalFacts.prop_extensionality.
+
+Open Scope Z_scope.
+
+(* destruct a list into elements when the length is a constant. *)
+Lemma Zlength_0_nil {A} : forall (al : list A),
+  Zlength al = 0 ->
+  al = nil.
+Proof.
+  intros. destruct al; list_solve.
+Qed.
+
+Lemma Zlength_gt_0_destruct {A} : forall (al : list A) n,
+  Zlength al = n ->
+  0 < n ->
+  exists x al', al = x :: al' /\ Zlength al' = n - 1.
+Proof.
+  intros.
+  destruct al; only 1 : list_solve.
+  assert (Zlength al = n - 1) by list_solve.
+  eauto.
+Qed.
+
+Lemma Zlength_lt_0_False {A} : forall (al : list A) n,
+  Zlength al = n ->
+  0 > n ->
+  False.
+Proof.
+  intros. list_solve.
+Qed.
+
+Ltac destruct_list xs :=
+  lazymatch goal with
+  | H : Zlength xs = ?n |- _ =>
+      let n' := eval compute in n in
+      lazymatch n' with
+      | Z0 => apply Zlength_0_nil in H; subst xs
+      | Zpos _ =>
+          first [ (* in case of H is used somewhere else *)
+            apply Zlength_gt_0_destruct in H; only 2 : reflexivity;
+            let xs' := fresh "xs" in
+            destruct H as [?x [xs' []]]; subst xs; destruct_list xs'
+          | let H' := fresh in
+            pose proof H as H';
+            apply Zlength_gt_0_destruct in H'; only 2 : reflexivity;
+            let xs' := fresh "xs" in
+            destruct H' as [?x [xs' []]]; subst xs; destruct_list xs'
+          ]
+      | Zneg _ =>
+          first [ (* in case of H is used somewhere else *)
+            apply Zlength_lt_0_False in H; only 2 : reflexivity;
+            inversion H
+          | let H' := fresh in
+            pose proof H as H';
+            apply Zlength_lt_0_False in H'; only 2 : reflexivity;
+            inversion H'
+          ]
+      end
+  | _ =>
+      idtac "Length of" xs "is not found"
+  end.
